Logic/IntProp/Kripke/LEM.lean
@@ -49,7 +49,7 @@ lemma noLEM_on_frameclass : ∃ (p : Formula α), ¬((Kripke.FrameClassOfHilbert
 /--
   Law of Excluded Middle is not always provable in intuitionistic logic.
 -/
-theorem noLEM : ∃ (p : Formula α), 𝐈𝐧𝐭 ⊬! p ⋎ ∼p := by
+theorem noLEM : ∃ (p : Formula α), 𝐈𝐧𝐭 ⊬ p ⋎ ∼p := by
   obtain ⟨p, hp⟩ := noLEM_on_frameclass (α := α);
   use p;
   by_contra hC;
@@ -87,7 +87,7 @@ lemma noLEM_on_frameclass_KC : ∃ (p : Formula α), ¬((Kripke.FrameClassOfHilb
     . simp;
     . simp [ValidOnModel, Satisfies];
 
-lemma noLEM_KC: ∃ (p : Formula α), 𝐊𝐂 ⊬! p ⋎ ∼p := by
+lemma noLEM_KC: ∃ (p : Formula α), 𝐊𝐂 ⊬ p ⋎ ∼p := by
   obtain ⟨p, hp⟩ := noLEM_on_frameclass_KC (α := α);
   use p;
   by_contra hC;
@@ -123,7 +123,7 @@ lemma noLEM_on_frameclass_LC : ∃ (p : Formula α), ¬((Kripke.FrameClassOfHilb
     . simp;
     . simp [ValidOnModel, Satisfies];
 
-lemma noLEM_LC: ∃ (p : Formula α), 𝐋𝐂 ⊬! p ⋎ ∼p := by
+lemma noLEM_LC: ∃ (p : Formula α), 𝐋𝐂 ⊬ p ⋎ ∼p := by
   obtain ⟨p, hp⟩ := noLEM_on_frameclass_LC (α := α);
   use p;
   by_contra hC;
